examples/AutoRewrite/AutoSetoidRewrite.v
@@ -1,0 +1,240 @@
+Require Import Coq.PArith.BinPos.
+Require Import Coq.Relations.Relations.
+Require Import Coq.FSets.FMapPositive.
+Require Import ExtLib.Core.RelDec.
+Require Import ExtLib.Data.Positive.
+Require Import ExtLib.Recur.Relation.
+Require Import ExtLib.Recur.GenRec.
+Require Import ExtLib.Tactics.
+Require Import MirrorCore.TypesI.
+Require Import MirrorCore.SymI.
+Require Import MirrorCore.EnvI.
+Require Import MirrorCore.Lambda.Expr.
+Require Import MirrorCore.Lambda.ExprD.
+Require Import MirrorCore.Lambda.ExprTac.
+
+Set Implicit Arguments.
+Set Strict Implicit.
+
+Section setoid.
+  Context {typ : Type}.
+  Context {func : Type}.
+  Context {RType_typD : RType typ}.
+  Context {Typ2_Fun : Typ2 RType_typD Fun}.
+  Context {RSym_func : RSym func}.
+
+  (** Reasoning principles **)
+  Context {RTypeOk_typD : RTypeOk}.
+  Context {Typ2Ok_Fun : Typ2Ok Typ2_Fun}.
+  Context {RSymOk_func : RSymOk RSym_func}.
+  Variable Typ0_Prop : Typ0 _ Prop.
+  Context {RelDec_eq_typ : RelDec (@eq typ)}.
+  Context {RelDec_eq_func : RelDec (@eq func)}.
+
+  Let tyArr : typ -> typ -> typ := @typ2 _ _ _ _.
+
+  Variable Rbase : Type.
+  Variable Req : Rbase -> Rbase -> bool.
+
+  Inductive RG : Type :=
+  | RGinj (r : Rbase)
+  | RGrespects (l r : RG)
+  | RGany (n : positive).
+
+  Record rsubst :=
+  { mp : PositiveMap.tree RG
+  ; max : positive
+  }.
+  Definition rsubst_set (n : positive) (a : RG) (r : rsubst)
+  : option (RG * rsubst) :=
+    match PositiveMap.find n r.(mp) with
+      | None =>
+        Some (a, {| mp := PositiveMap.add n a r.(mp) ; max := r.(max) |})
+      | Some _ => None
+    end.
+
+  Definition rsubst_lookup (r : rsubst) n : option RG :=
+    PositiveMap.find n r.(mp).
+
+  Definition rsubst_empty : rsubst :=
+    {| mp := PositiveMap.empty _ ; max := 1 |}.
+
+  Section unifyRG.
+    Variable (unifyRG : RG -> RG -> rsubst -> option (RG * rsubst)).
+    Fixpoint unifyRG' (l r : RG) (env : rsubst)
+    : option (RG * rsubst) :=
+      match l , r with
+        | RGany n , RGany n' =>
+          if n ?[ eq ] n' then Some (l, env)
+          else match PositiveMap.find n env.(mp) with
+                 | None => rsubst_set n r env
+                 | Some l => match PositiveMap.find n' env.(mp) with
+                               | None => rsubst_set n' l env
+                               | Some _ => None
+                             end
+               end
+        | RGany n , _ =>
+          match PositiveMap.find n env.(mp) with
+            | None => rsubst_set n r env
+            | Some v => unifyRG v r env
+          end
+        | _ , RGany n =>
+          match PositiveMap.find n env.(mp) with
+            | None => rsubst_set n l env
+            | Some v => unifyRG l v env
+          end
+        | RGinj l , RGinj r =>
+          if Req l r then Some (RGinj l, env) else None
+        | RGrespects la lb , RGrespects ra rb =>
+          match unifyRG' la ra env with
+            | Some (l',env') =>
+              match unifyRG' ra rb env' with
+                | Some (r',env'') => Some (RGrespects l' r', env'')
+                | None => None
+              end
+            | None => None
+          end
+        | _ , _ => None
+      end.
+  End unifyRG.
+
+  Fixpoint unifyRG_ (n : nat) (l r : RG) (env : rsubst)
+  : option (RG * rsubst) :=
+    match n with
+      | 0 => None
+      | S n => unifyRG' (fun l r env => unifyRG_ n l r env) l r env
+    end.
+
+  Definition unifyRG := unifyRG_ 10.
+
+  Variable rw : expr typ func -> list RG -> RG -> rsubst ->
+                option (expr typ func * rsubst).
+  Variable rw_default : expr typ func -> list RG -> RG -> rsubst ->
+                        option (expr typ func * rsubst).
+
+  Definition rsubst_fresh (rs : rsubst) : (positive * rsubst) :=
+    (rs.(max), {| mp := rs.(mp) ; max := rs.(max) + 1 |}).
+
+  Fixpoint setoid_rewrite
+           (e : expr typ func) (rvars : list RG) (rg : RG) (rs : rsubst)
+  : option (expr typ func * rsubst).
+  refine (
+      match rw e rvars rg rs with
+        | None =>
+          match e with
+            | App f x =>
+              let (nxt,rs) := rsubst_fresh rs in
+              match setoid_rewrite f rvars (RGrespects (RGany nxt) rg) rs with
+                | None => None
+                | Some (f', rs') =>
+                  match setoid_rewrite x rvars (RGany nxt) rs' with
+                    | None => None
+                    | Some (x',rs'') => Some (App f' x',rs'')
+                  end
+              end
+            | Abs t b =>
+              match rg with
+                | RGrespects l r =>
+                  match setoid_rewrite b (l :: rvars) r rs with
+                    | None => None
+                    | Some (b',rs') =>
+                      Some (Abs t b', rs')
+                  end
+                | RGany n =>
+                  match rsubst_lookup rs n with
+                    | None =>
+                      let (l,rs) := rsubst_fresh rs in
+                      let (r,rs) := rsubst_fresh rs in
+                      match rsubst_set n (RGrespects (RGany l) (RGany r)) rs with
+                        | None => None (* DEAD *)
+                        | Some (_,rs') =>
+                          match setoid_rewrite b (RGany l :: rvars) (RGany r) rs' with
+                            | None => None
+                            | Some (b',rs') => Some (Abs t b',rs')
+                          end
+                      end
+                    | Some (RGrespects l r) =>
+                      match setoid_rewrite b (l :: rvars) r rs with
+                        | None => None
+                        | Some (b',rs') =>
+                          Some (Abs t b', rs')
+                      end
+                    | _ => None
+                  end
+                | _ => None
+              end
+            | Var v =>
+              match nth_error rvars v with
+                | None => None (** Dead code **)
+                | Some r =>
+                  match unifyRG r rg rs with
+                    | None => rw_default e rvars rg rs
+                    | Some (r',rs') =>
+                      Some (Var v, rs')
+                  end
+              end
+            | Inj _ => rw_default e rvars rg rs
+            | UVar u => rw_default e rvars rg rs
+          end
+        | Some x => Some x
+      end).
+  Defined.
+
+  (*
+  (** This will be called on the head symbol to see what it
+   ** respects
+   **)
+  Variable respects : expr typ func -> RG -> option RG.
+  Variable is_reflexive : RG -> option RG.
+
+  Definition try_reflexive (e : expr typ func)
+             (rvars : list RG) (rg : RG)
+  : option (expr typ func * list RG * RG) :=
+    match is_reflexive rg with
+      | None => None
+      | Some r => Some (e, rvars, r)
+    end.
+*)
+
+  Inductive R : Type :=
+  | Rinj (r : Rbase)
+  | Rrespects (l r : R).
+
+  Fixpoint RtoRG (r : R) : RG :=
+    match r with
+      | Rinj r => RGinj r
+      | Rrespects l r => RGrespects (RtoRG l) (RtoRG r)
+    end.
+
+  Fixpoint findRewrite (ls : list (expr typ func * RG * expr typ func))
+           (e : expr typ func) (rg : RG) (rs : rsubst)
+  : option (expr typ func * rsubst) :=
+    match ls with
+      | nil => None
+      | (l,R,r) :: ls =>
+        if l ?[ eq ] e then
+          match unifyRG R rg rs with
+            | None => findRewrite ls e rg rs
+            | Some (_,rs') => Some (r,rs')
+          end
+        else
+          findRewrite ls e rg rs
+    end.
+
+  Definition fromRewrites (ls : list (expr typ func * R * expr typ func))
+  : forall (e : expr typ func) (rvars : list RG) (rg : RG) (rs : rsubst),
+      option (expr typ func * rsubst) :=
+    let ls := map (fun x => let '(a,b,c) := x in
+                            (a,RtoRG b, c)) ls in
+    fun e rvars => findRewrite ls e.
+
+  Definition fromReflexive (is_refl : RG -> rsubst -> option rsubst)
+  : forall (e : expr typ func) (rvars : list RG) (rg : RG) (rs : rsubst),
+      option (expr typ func * rsubst) :=
+    fun e rvars rg rs =>
+      match is_refl rg rs with
+        | None => None
+        | Some rs' => Some (e, rs')
+      end.
+
+End setoid.
