examples/AutoRewrite/DemoAutoSetoidRewrite.v
@@ -1,0 +1,103 @@
+Require Import ExtLib.Core.RelDec.
+Require Import MirrorCore.Lambda.ExprCore.
+Require Import MirrorCore.Lambda.ExprD.
+Require Import McExamples.AutoRewrite.AutoSetoidRewrite.
+Require Import McExamples.Simple.Simple.
+
+Set Implicit Arguments.
+Set Strict Implicit.
+
+Require Import McExamples.Simple.Simple.
+
+Let Rbase := expr typ func.
+
+Definition m (T : Type) : Type :=
+  rsubst Rbase -> option (T * rsubst Rbase).
+
+Definition rg_bind {T U} (a : m T) (b : T -> m U) : m U :=
+  fun s => match a s with
+             | None => None
+             | Some (val,s') => b val s'
+           end.
+Definition rg_fail {T} : m T := fun _ => None.
+Definition rg_ret {T} (v : T) : m T := fun s => Some (v, s).
+Definition rg_plus {T} (l r : m T) : m T :=
+  fun s =>
+    let v := l s in
+    match v with
+      | None => r s
+      | Some _ => v
+    end.
+
+Definition SRrespects (e : expr typ func) (l : RG (expr typ func))
+: m (RG (expr typ func)) :=
+  match e , l with
+    | Inj Lt , RGrespects a (RGrespects b (RGinj (Inj (Eq _)))) =>
+      rg_bind
+        (unifyRG (fun x y => x ?[ eq ] y) a (RGinj (Inj Lt)))
+        (fun a =>
+           rg_bind
+             (unifyRG (fun x y => x ?[ eq ] y) b (RGinj (Inj (Eq tyNat))))
+             (fun b =>
+                rg_ret (RGrespects a (RGrespects b (RGinj (Inj (Eq tyProp)))))))
+    | Inj (Eq t) , RGrespects a (RGrespects b (RGinj (Inj (Eq _)))) =>
+      rg_bind
+        (unifyRG (fun x y => x ?[ eq ] y) a (RGinj (Inj (Eq t))))
+        (fun a =>
+           rg_bind
+             (unifyRG (fun x y => x ?[ eq ] y) b (RGinj (Inj (Eq t))))
+             (fun b =>
+                rg_ret (RGrespects a (RGrespects b (RGinj (Inj (Eq t)))))))
+    | Inj Plus , RGrespects a (RGrespects b (RGinj (Inj (Eq t)))) =>
+      rg_bind
+        (unifyRG (fun x y => x ?[ eq ] y) a (RGinj (Inj (Eq t))))
+        (fun a =>
+           rg_bind
+             (unifyRG (fun x y => x ?[ eq ] y) b (RGinj (Inj (Eq t))))
+             (fun b =>
+                rg_ret (RGrespects a (RGrespects b (RGinj (Inj (Eq t)))))))
+    | _ , _ => rg_fail
+  end.
+
+Let plus_expr : expr typ func := (App (App (Inj Plus) (Inj (N 0))) (Inj (N 5))).
+
+Definition the_rewriter (e : expr typ func) (c : list (RG (expr typ func)))
+           (rg : RG (expr typ func))
+: m (expr typ func) :=
+  match e with
+    | Inj (N 0) =>
+      rg_bind (unifyRG (fun x y => x ?[ eq ] y) rg (RGinj (Inj (Eq tyNat))))
+              (fun _ =>
+                 rg_ret (Inj (N 1)))
+    | Inj _ => rg_bind (SRrespects e rg) (fun _ => rg_ret e)
+    | _ => rg_fail
+  end.
+
+Definition rewriter (e : expr typ func)
+           (vars : list (RG Rbase))
+           (r : RG Rbase) : m (expr typ func) :=
+  the_rewriter e vars r.
+
+Definition rewriter_default (e : expr typ func)
+           (vars : list (RG Rbase))
+           (rg : RG Rbase) : m (expr typ func) :=
+  match rg with
+    | RGany n =>
+      let type := tyNat in
+      rg_bind
+        (unifyRG (fun x y => x ?[ eq ] y) rg (RGinj (Inj (Eq type))))
+        (fun _ => rg_ret e)
+    | RGinj (Inj (Eq _)) => rg_ret e
+    | _ => rg_fail
+  end.
+
+
+
+Eval vm_compute in
+    @setoid_rewrite typ func (expr typ func)
+                    (fun x y => x ?[ eq ] y)
+                    rewriter
+                    rewriter_default
+                    plus_expr
+                    (RGinj (Inj (Eq tyNat)) :: RGinj (Inj (Eq tyNat)) :: nil)
+                    (RGinj (Inj (Eq tyNat))) (@rsubst_empty _).
